\documentclass[a4paper,10pt]{article}
\usepackage[a4paper, hmargin={1.5cm,1.5cm}, vmargin={1.5cm,1.5cm}]{geometry}
\usepackage{amsmath}
\usepackage{amssymb}
\usepackage{amsthm}
\usepackage{amsfonts}
\usepackage{color}
\usepackage{graphicx}

\newcommand{\R}{\mathbb{R}}
\newcommand{\N}{\mathbb{N}}

\title{Report Topics in Computational Science}
\author{Afifah Maya Iknaningrum \\ 1715011053}

\begin{document}
	\maketitle
	
\textbf{Problem 1 :} \\ Let $ m>1 $ and suppose that $ u $ is a twice continuously differentiable positive solution in the pressure porous medium equation
\begin{equation}\label{porous_1}
u_{t}- \Delta(u^{m}) =0 ,  \ x\in \R , t>0.
\end{equation}
Show that $ p(x,t):=\dfrac{m}{m-1}u^{m-1}(x,t) $ is a solution of the porous medium equation in the pressure form
\begin{equation}\label{porous_2}
p_{t}-(m-1)p\Delta p-|\nabla p|^2 = 0
\end{equation}

\textbf{Answer 1 :} \\ Substitute 
\begin{equation}\label{p}
p(x,t):=\dfrac{m}{m-1}u^{m-1}(x,t)
\end{equation} 
, to equation (\ref{porous_2}), we obtain
\begin{eqnarray}\nonumber
&&p_{t}-(m-1)p\Delta p-|\nabla p|^2 \\ \nonumber
&=&\Big( \dfrac{m}{m-1}(m-1)u^{m-2}u_{t} \Big) - \Big( (m-1)\dfrac{m}{m-1} u^{m-1}m(m-2)u^{m-3}u_{x}^{2}+m^{2}u^{m-2}u_{xx} \Big) - |mu^{m-2}u_{x}|^{2} \\ \label{eq1}
&=& mu^{m-2}u_{t} - (m^{3}+m^{2}-2m)u^{2m-4}u_{x}^{2}-m^{3}u^{2m-3}u_{xx}
\end{eqnarray}
Remember we have
\begin{equation}\label{eq2}
u_{t}-\Delta(u^{m}) = u_{t}-(m^2-m)u^{m-2}u_{x}^{2}-m^{2}u^{m-1}u_{xx}= 0.
\end{equation}

Then the equation (\ref{eq1}) can be modified such that it is contain equation (\ref{eq2}) such that
\begin{eqnarray}\nonumber
&&mu^{m-2}u_{t} - (m^{3}+m^{2}-2m)u^{2m-4}u_{x}^{2}-m^{3}u^{2m-3}u_{xx}\\ \nonumber
&=&mu^{m-2}\big( u_{t}-(m^2-m)u^{m-2}u_{x}^{2}-m^{2}u^{m-1}u_{xx} \big)+\big((m^3-m^2)-(m^3-2m^2)-m^2 \big)u^{2m-4}u_{x}^{2}+(m^3-m^3)u^{2m-3}u_{xx}\\ \nonumber
&=& 0
\end{eqnarray}
It is shown that $ p(x,t) $ as defined above, is a solution of the porous medium equation in the pressure form (\ref{porous_2}).

\newpage
\textbf{Problem 2 :} \\ For dimension $ n\in \N $ and constant $ m>1,C>0,\alpha>0,\beta>0 $. Define the function $ u: \R^n \times (0,\infty) \rightarrow \R$ as
\[ u(x,t) = t^{-\alpha}\Big( \max \big( C-\dfrac{\beta(m-1)}{2m} \dfrac{|x|^2}{t^{2\beta}} , 0 \big) \Big)^{\frac{1}{m-1}}, \ x\in \R^n, t>0 \]
where $ |x|:=(\sum_{i=1}^{n} x_{i}^{2})^{1/2} $
\begin{enumerate}
	\item Find $ \alpha $ and $ \beta $ in terms of $ m $ and $ n $ so that $ u $ is a solution of (\ref{porous_1}) in the set
	\[ \{ (x,t): x\in \R^n, t>0, u(x,t)>0\}. \]
	
	\textbf{Answer :}
	We have $ p $ as defined in (\ref{p}). Because the set, we should take $ u(x,t)>0 $ such that
	\begin{eqnarray}\nonumber
	u(x,t) &=& t^{-\alpha}\big( C-\dfrac{\beta(m-1)}{2m} \dfrac{|x|^2}{t^{2\beta}} \big)^{\frac{1}{m-1}} \\ \nonumber
	p(x,t) &=& \dfrac{m}{m-1} t^{-\alpha(m-1)}\big( C-\dfrac{\beta(m-1)}{2m} \dfrac{|x|^2}{t^{2\beta}} \big)\\ \nonumber
	p_{t}(x,t) &=& -\alpha m t^{-\alpha(m-1)-1}\big( C-\dfrac{\beta(m-1)}{2m} \dfrac{|x|^2}{t^{2\beta}} \big)^{\frac{1}{m-1}} +  \beta^2 |x|^2 t^{-\alpha(m-1)-2\beta-1} \\ \nonumber
	&=& -\dfrac{\alpha}{t} (m-1)p(x,t) +  \beta^2 |x|^2 t^{-\alpha(m-1)-2\beta-1}\\ \nonumber
	\nabla p(x,t) &=& -\beta t^{-\alpha(m-1)-2\beta} x \\ \nonumber
	\Delta p(x,t) &=& -\beta t^{-\alpha(m-1)-2\beta} n
	\end{eqnarray}
	From the information we had above, we can subtitute it to (\ref{porous_2}) such that
	\begin{eqnarray}\nonumber
	&& p_{t}-(m-1)p\Delta p-|\nabla p|^2 \\ \nonumber
	&=& \Big(-\dfrac{\alpha}{t} (m-1)p(x,t) +  \beta^2 |x|^2 t^{-\alpha(m-1)-2\beta-1}\Big)-\Big((m-1)p(x,t)\big(-\beta t^{-\alpha(m-1)-2\beta} n\big)  \Big) - |\big(-\beta t^{-\alpha(m-1)-2\beta} x\big)|^{2} \\ \nonumber
	&=& \Big( -\dfrac{\alpha}{t} + \beta n t^{-\alpha(m-1)-2\beta} \Big)(m-1)p(x,t) + \beta^2|x|^2\Big( t^{-\alpha(m-1)-2\beta-1}-t^{-2\alpha(m-1)-4\beta} \Big)\\ \nonumber
	&=& 0
	\end{eqnarray}
	Because $ \alpha,\beta,t,C>0 \ , \ m>1$ and by $ u(x,t)>0 $, then $ p(x,t) >0 $. Then to make the equation above holds. We can let
	\begin{eqnarray}\nonumber
	&-\alpha t^{-1} + \beta n t^{-\alpha(m-1)-2\beta} &=0 \\ \nonumber
	\Leftrightarrow & \alpha t^{-1} &= \beta n t^{-\alpha(m-1)-2\beta} \\ \nonumber
	\Leftrightarrow & \alpha = \beta n &\text{ and } t^{-1} = t^{-\alpha(m-1)-2\beta}\\ \nonumber
	\Leftrightarrow &\alpha = \beta n &\text{ and }  \beta = \dfrac{1}{n(m-1)+2}\\ \nonumber
	\Leftrightarrow &\alpha = \dfrac{n}{n(m-1)+2} &\text{ and }  \beta = \dfrac{1}{n(m-1)+2}
	\end{eqnarray}
	Substitute $ \alpha $ and $ \beta $ we obtain into
	\begin{eqnarray}\nonumber
	&t^{-\alpha(m-1)-2\beta-1}-t^{-2\alpha(m-1)-4\beta} &= 0 \\ \nonumber
	\Leftrightarrow& -\alpha(m-1)-2\beta-1 &= -2\alpha(m-1)-4\beta \\ \nonumber
	\Leftrightarrow& -\dfrac{n}{n(m-1)+2}(m-1)-2\dfrac{1}{n(m-1)+2}-1 &= -2 \dfrac{n}{n(m-1)+2}(m-1)-4\dfrac{1}{n(m-1)+2} \\ \nonumber
	\Leftrightarrow& -n(m-1)-2-(n(m-1)+2) &= -2n(m-1)-4 \\ \nonumber
	\Leftrightarrow& -2nm+2n-4 &= -2nm+2n-4
	\end{eqnarray}
	So the $ \alpha = \dfrac{n}{n(m-1)+2} \text{ and }  \beta = \dfrac{1}{n(m-1)+2} $ we got is satisfy the $ u $ solution of (\ref{porous_1}).
	\newpage
	\item For given $ t>0 $, the set $ \Omega(t):=\{ x\in\R^n: u(x,t)>0 \} $ is an $ n $-dimensional ball. Find its radius $ r=r(t) $. Find $ \lim\limits_{t\rightarrow 0+}r(t) $ and $ \lim\limits_{t\rightarrow \infty} r(t) $.\\ \\
	\textbf{Answer :}\\ 
	Because of the definition of $ \Omega(t) $, then we take
	\[ u(x,t) = t^{-\alpha}\big( C-\dfrac{\beta(m-1)}{2m} \dfrac{|x|^2}{t^{2\beta}} \big)^{\frac{1}{m-1}} \]
	Then, $ u(x,t) $ should be positive for $ x\in \R^n $ such that
	\[ u(-x,t) = u(x,t). \]
	So we can see that the center of ball is $ 0 $ and the $ |x| = r $. To find the radius, we can use the fact that
	\begin{eqnarray} \nonumber
	&C-\dfrac{\beta(m-1)}{2m} \dfrac{r^2}{t^{2\beta}} &= 0 \\ \nonumber
	\Leftrightarrow&\dfrac{r^2}{t^{2\beta}} &= \dfrac{2Cm}{\beta(m-1)} \\ \nonumber
	\Leftrightarrow& r(t) &= \sqrt{\dfrac{2Cmt^{2\beta}}{\beta(m-1)}}	
	\end{eqnarray}
	We could find
	\[ \lim\limits_{t\rightarrow 0+}r(t) = \lim\limits_{t\rightarrow 0+}\sqrt{\dfrac{2Cmt^{2\beta}}{\beta(m-1)}} = 0 \]
	and
	\[ \lim\limits_{t\rightarrow \infty}r(t) = \lim\limits_{t\rightarrow \infty}\sqrt{\dfrac{2Cmt^{2\beta}}{\beta(m-1)}} = \infty \]
	\newpage
	\item For $ n=2 $ and the constants $ \alpha $ and $ \beta $ from (1), compute the value of
	\[ M(t) := \int_{\R^n} u(x,t) \ dx \]
	for $ t>0 $. Does the solution conserve mass $ M(t) $ ?\\ \\
	\textbf{Answer :} \\ 
	\begin{eqnarray}\nonumber
	M(t) &:=& \int_{\R^2} u(x,t) \ dx \\ \nonumber
	&=& \int_{x_{1}} \int_{x_{2}} u(x,t) \ dx_{1}dx_{2} \\ \nonumber
	&=& \int_{\theta} \int_{r}  r t^{-\alpha}\big( C-\dfrac{\beta(m-1)}{2m} \dfrac{r^2}{t^{2\beta}} \big)^{\frac{1}{m-1}} \ dr d\theta \\ \nonumber
	&=& \int_{0}^{2\pi} \int_{0}^{r(t)}  t^{-\alpha}\big( Cr-\dfrac{\beta(m-1)}{2m} \dfrac{r^3}{t^{2\beta}} \big)^{\frac{1}{m-1}} \ dr d\theta \\ \nonumber
	&=& t^{-\alpha}  \int_{0}^{2\pi} \Big[ \dfrac{Cr^2}{2} - \dfrac{\beta(m-1)r^4}{8mt^{2\beta}} \Big]_{0}^{r(t)} d\theta \\ \nonumber
	&=& t^{-\alpha}  \int_{0}^{2\pi} \dfrac{C\big(\dfrac{2Cmt^{2\beta}}{\beta(m-1)}\big)}{2} - \dfrac{\beta(m-1)\big(\dfrac{2Cmt^{2\beta}}{\beta(m-1)}\big)^2}{8mt^{2\beta}}  d\theta \\ \nonumber
	&=& t^{-\alpha} \int_{0}^{2\pi} \dfrac{C^2mt^{2\beta}}{2\beta(m-1)} d\theta \\ \nonumber
	&=& t^{-\alpha} \pi \dfrac{C^2mt^{2\beta}}{\beta(m-1)} 
	\end{eqnarray}
	Substitute $ \alpha = \dfrac{n}{n(m-1)+2} \text{ and }  \beta = \dfrac{1}{n(m-1)+2} $ we got
	\[ M(t) = \Big(t^{-\big(\dfrac{n}{n(m-1)+2}\big)} \pi\Big) \Big(\dfrac{C^2mt^{2\big(\dfrac{1}{n(m-1)+2}\big)}}{\big(\dfrac{1}{n(m-1)+2}\big)(m-1)}\Big) = \dfrac{2C^2m^2\pi}{m-1} \]
	As we can see, $ M(t) $ is constant and independent of $ t $, so the solution is conserve mass $ M(t) $.
\end{enumerate}

\end{document}